Finished up subtask e, only debugging remains

LimitedStack.dfy
@@ -2,74 +2,79 @@
 class LimitedStack{
 
       var capacity : int; // capacity, max number of elements allowed on the stack.
-      var arr : array<int>; // contents of stack.
+      var arr : array?<int>; // contents of stack.
       var top : int; // The index of the top of the stack, or -1 if the stack is empty
 
       // This predicate express a class invariant: All objects of this calls should satisfy this.
       predicate Valid()
-      reads ?;
+      reads this;
       {
-        
+          arr != null && capacity > 0 && capacity == arr.Length && top >= -1 && top < capacity
       }
 
       predicate Empty()
       reads this;
       {
-        
+          top == -1
       }
 
       predicate Full()
       reads this;
       {
-        
+          top == capacity - 1
       }
- /*     
+
       method Init(c : int)
       modifies this;
-      requires ? 
+      requires c > 0;
 
       ensures fresh(arr); // ensures arr is a newly created object.
-      // Additional post-condition to be given here!
+      ensures Valid();
+      ensures Empty();
+
       {
         capacity := c;
         arr := new int[c];
         top := -1;
       }
-*/
 
-/*      
+     
       method isEmpty() returns (res : bool)
-      
+      requires Empty();
       {
-        
+            res := true;
       }
-*/
 
-/*
+
       // Returns the top element of the stack, without removing it.
       method Peek() returns (elem : int)
-      
+      requires Valid();
+      requires !Empty();
       {
-        
+          elem := arr[top];
       }
-*/
 
-/*
       // Pushed an element to the top of a (non full) stack. 
       method Push(elem : int)
-      
+      requires Valid();
+      requires !Full();
+
+      modifies this.arr, this`top;
       {
-        
+          top := top + 1;
+          arr[top] := elem;
       }
-*/
+
       // Pops the top element off the stack.
-/*  
       method Pop() returns (elem : int)
-      
+        requires Valid();
+        requires !Empty();
+
+        modifies this`top;
       {
-        
+          elem := arr[top];
+          top := top-1;
       }
- */
  
       method Shift()
       requires Valid() && !Empty();
@@ -91,16 +96,19 @@ class LimitedStack{
         top := top - 1;
       }
 
-/*
       //Push onto full stack, oldest element is discarded.
       method Push2(elem : int)
-      
-      {
-        
-      }
-*/
+      requires Valid();
 
-/*
+      modifies this.arr, this`top;
+      {
+            if(top == capacity-1) {
+                Shift();
+            }
+            top := top+1;
+            arr[top] := elem;
+      }
+
 
 // When you are finished,  all the below assertions should be provable. 
 // Feel free to add extra ones as well.
@@ -133,5 +141,4 @@ class LimitedStack{
            assert s.arr[0] == 32;
                      
        }
-*/
 }
